Vec.seq sound lemma and some Vec.lean cleanup

Translation/Global.lean
@@ -15,18 +15,18 @@ def Surface.Ty.translate_ctors (G : Core.GlobalEnv) (ctors : Vect n  (String × 
   -- check that names are unique
   let cns : Vect n String := (λ x => x.1) <$> ctors
 
-  let octors' : Vect n (Option (String × Core.Ty)) :=  (λ (x, ty) =>
-    do let ty' : Core.Ty <- ty.translate
-       let _ <- Core.is_valid_ctor_ty G ty'
+  let octors : Vect n (Option (String × Core.Ty)) :=  (λ (x, ty) =>
+    do let ty' := ty.translate
+       Core.is_valid_ctor_ty G ty'
        return (x , ty')) <$> ctors
-  octors'.seq
+  octors.seq
 
 
 
 @[simp]
 def Surface.Global.translate (G : Core.GlobalEnv) : Global -> Option Core.Global
 | .data (n := n) x K ctors => do
-  let ctors' <- Ty.translate_ctors G ctors
+  let ctors' <- Ty.translate_ctors ((Core.Global.data 0 x K.translate Vect.nil) :: G) ctors
   return Core.Global.data n x K.translate ctors'
 
 @[simp]
@@ -36,3 +36,15 @@ def Surface.GlobalEnv.translate : Surface.GlobalEnv -> Option (Core.GlobalEnv)
   let gs' <- Surface.GlobalEnv.translate gs
   let g' <- g.translate gs'
   return g' :: gs'
+
+
+namespace Test.Core.Global
+
+
+def t := ([ ("1" , gt`#"One")] : Vect 1 (String × Surface.Ty))
+
+#eval (gt`#"One").translate
+
+-- #eval Surface.Ty.translate_ctors [] t
+
+end Test.Core.Global
