Translation/Rename.lean
@@ -32,10 +32,29 @@ theorem Translation.Ty.Weaken {T : Surface.Ty} {T' : Core.Ty} :
 intro h; apply Translation.Ty.Rename (λ x => x + 1) h
 
 
+theorem Subst.Surface.Ty.translate_commute_lift {σ : Subst Surface.Ty} :
+  Subst.Surface.Ty.translate σ.lift =
+    re 0 :: Subst.Surface.Ty.translate σ ∘ +1 := by
+funext; case _ x =>
+induction x generalizing σ
+case zero => simp
+case succ n ih =>
+ simp only [translate, Subst.lift];
+ generalize zdef : σ n = z at *
+ cases z <;> simp
+ case re => simp [Subst.compose,translate,zdef]
+ case su T =>
+ have e := Translation.Ty.Weaken (T := T) rfl; simp at e
+ simp [Subst.compose, translate, zdef]; rw[<-e];
+ simp[<-Ren.to_succ, rmap, smap]; simp;
+ have lem0 := Surface.Ty.apply_stable (λ x => x + 1) (+1) rfl;
+ have lem : Surface.Ty.rmap (fun x => x + 1) T = Surface.Ty.smap +1 T := by rw[lem0]
+ rw[lem]
+
 theorem Translation.Ty.Subst (σ : Subst Surface.Ty)
   {T : Surface.Ty} {T' : Core.Ty} :
   T.translate = T' ->
-  (T[σ]).translate = T'[Subst.Surface.Ty.translate σ] := by
+  ⟦T[σ]⟧ = T'[⟦σ⟧] := by
 intro h1
 fun_induction Surface.Ty.translate generalizing T' σ <;> (subst h1; simp at *)
 case _ x =>
@@ -49,6 +68,6 @@ case _ ih1 ih2 =>
 )
 case _ k p ih =>
   replace ih := ih σ.lift
-  have lem := Subst.Surface.Ty.translate_compose (σ := σ)
+  have lem := Subst.Surface.Ty.translate_commute_lift (σ := σ)
   simp at lem ih
   rw[ih, lem]
